new equiv

proof/spec/XMSS_vs_XMSS_MT.ec
@@ -5,34 +5,12 @@ import IntID.
 
 require import Array8.
 
-abbrev eqsk (sk : xmss_sk, skmt : xmss_mt_sk) : bool = 
-    sk.`idx = skmt.`idx /\
-    sk.`sk_seed = skmt.`sk_seed /\
-    sk.`sk_prf = skmt.`sk_prf /\
-    sk.`pub_seed_sk = skmt.`pub_seed_sk /\
-    sk.`sk_root = skmt.`sk_root. 
 
-abbrev eqpk (pk : xmss_pk, pkmt : xmss_mt_pk) : bool = 
-    pk.`pk_oid = pkmt.`pk_oid /\
-    pk.`pk_root = pkmt.`pk_root /\
-    pk.`pk_pub_seed = pkmt.`pk_pub_seed. 
-
-abbrev eqkp (kp : xmss_keypair, kpmt : xmss_mt_keypair) : bool = 
-    kp.`1.`idx = kpmt.`1.`idx /\
-    kp.`1.`sk_seed = kpmt.`1.`sk_seed /\
-    kp.`1.`sk_prf = kpmt.`1.`sk_prf /\
-    kp.`1.`pub_seed_sk = kpmt.`1.`pub_seed_sk /\
-    kp.`1.`sk_root = kpmt.`1.`sk_root /\
-    kp.`2.`pk_oid = kpmt.`2.`pk_oid /\
-    kp.`2.`pk_root = kpmt.`2.`pk_root /\
-    kp.`2.`pk_pub_seed = kpmt.`2.`pk_pub_seed. 
-
-
-equiv keygen : XMSS_PRF.kg ~ XMSS_MT_PRF.kg : XMSS_Params.impl_oid = XMSS_MT_Params.impl_oid /\ d = 1 ==> eqkp res{1} res{2}. 
+equiv keygen : XMSS_PRF.kg ~ XMSS_MT_PRF.kg : XMSS_Params.impl_oid = XMSS_MT_Params.impl_oid /\ d = 1 ==> ={res}. 
 proof. 
-proc. wp 11 11 => /=. 
+proc. wp 7 7 => /=.
 call(:d=1);1: by conseq />; sim; auto => /> /#.
-wp 9 9 => /=. 
+wp 5 5 => /=. 
 call(:d=1);1: by conseq />; sim. 
 by auto => /> /#.
 qed.
@@ -40,17 +18,17 @@ qed.
 abbrev eqsig(sig : XMSS_Types.sig_t, sigmt : XMSS_MT_Types.sig_t) : bool =
    sig.`sig_idx = sigmt.`sig_idx /\
    sig.`r = sigmt.`r /\
-   sig.`r_sigs = sigmt.`r_sigs.
+   [sig.`r_sig] = sigmt.`r_sigs.
 
 equiv sign : XMSS_PRF.sign ~ XMSS_MT_PRF.sign : 
     XMSS_Params.impl_oid = XMSS_MT_Params.impl_oid /\  
     d=1 /\ 
     h < 32 /\ 0 < to_uint sk{2}.`idx < 2^h - 1 /\ 
-    eqsk arg{1}.`1 arg{2}.`1 /\ arg{1}.`2 = arg{2}.`2 ==> 
-     eqsig res{1}.`1 res{2}.`1 /\ eqsk res{1}.`2 res{2}.`2. 
+    arg{1}.`1 = arg{2}.`1 /\ arg{1}.`2 = arg{2}.`2 ==> 
+     eqsig res{1}.`1 res{2}.`1 /\ res{1}.`2 = res{2}.`2. 
 proof. 
 proc => /=. 
-rcondf {2} 22.
+rcondf {2} 18.
 + move => ?.
   wp;call(:true);1:by trivial.
   wp;call(:true);1:by trivial.
@@ -64,38 +42,33 @@ call(: d=1 /\ ={arg} /\ 0 < to_uint idx{1} /\ to_uint idx{2} < 2 ^ h - 1 ==> ={r
   wp => /=. 
   call(: d=1 /\ ={arg} /\ 0 < to_uint idx{1} /\ to_uint idx{2} < 2 ^ h - 1 ==> ={res}).
   +  proc => /=. 
-     while (#post /\ d = 1 /\ ={pub_seed,sk_seed,t,j,idx} /\ 0 <= j{1} <= h /\
-       0 < to_uint idx{1} /\ to_uint idx{2} < 2 ^ h - 1).
-     + auto => />;conseq (: ={j,t,address}). smt(). 
+     while (#post /\ d = 1 /\ ={authentication_path, pub_seed,sk_seed,t,j,idx} /\ 0 <= j{1} <= h /\
+       0 < to_uint idx{1} /\ to_uint idx{2} < 2 ^ h - 1). 
+     + auto => />; conseq (:  ={authentication_path, j,t,address});1:smt().
      call(:d=1); 1: by conseq />;sim;auto => /> /#.
      by auto => />.
-   by auto => />;1: by smt(ge0_h).
+   by auto => />; 1: by smt(ge0_h).
 by auto => />.
 
 wp;call(:true); 1: by sim.
-auto => /> &1 &2 ? -> /= *;split;1:smt(). 
-move => *; do split;1: smt(). 
+auto => /> &1 ? -> /= *; do split. 
 + rewrite and_mod;1:smt(ge0_h).
   by rewrite modz_small /=; smt(). 
 + rewrite /zero_address /set_tree_addr /set_layer_addr  to_uint_shr /=; 1: by smt(ge0_h). 
-  have -> : (to_uint sk{2}.`idx %/ 2 ^ h) = 0 by smt().
+  have -> : (to_uint sk{1}.`idx %/ 2 ^ h) = 0 by smt().
   apply tP => i ib.
   rewrite !initiE 1:/# /=.
   rewrite !get_setE 1..3:/#.
   by rewrite initiE 1:/# /=.
 
-+ by smt().
-
 + rewrite and_mod;1:smt(ge0_h).
   by rewrite modz_small /=; smt(). 
-
-by smt().
 qed.
 
 equiv verify : XMSS_PRF.verify ~ XMSS_MT_PRF.verify : 
     d=1 /\ 
     h < 32 /\ 0 < to_uint s{2}.`sig_idx < 2^h - 1 /\ 
-    eqpk arg{1}.`1 arg{2}.`1 /\ arg{1}.`2 = arg{2}.`2 /\ eqsig arg{1}.`3 arg{2}.`3 ==> ={res}.
+    arg{1}.`1 = arg{2}.`1 /\ arg{1}.`2 = arg{2}.`2 /\ eqsig arg{1}.`3 arg{2}.`3 ==> ={res}.
 proc.
 rcondf {2} 16.
 + move => ?.
@@ -103,11 +76,11 @@ rcondf {2} 16.
   by auto => /> /#.
 wp;call(: true); 1: by sim.
 auto => /> &1 &2 -> /=.
-move => *; do split.
+move => /> H H0 H1 H2 H3 H4; do split.
 + rewrite W32.and_mod /=;1:smt(ge0_h).
   by rewrite modz_small /=; 1:smt().
-+ by smt().
-+ by smt().
++ rewrite -H4 /=;by smt().
++ rewrite -H4 /=;by smt().
 + by smt().
 
 + rewrite to_uint_shr;1:smt(ge0_h).
@@ -117,6 +90,4 @@ move => *; do split.
   rewrite !initiE 1:/# /=.
   rewrite !get_setE 1..3:/#.
   by rewrite initiE 1:/# /=.
-
-by smt().
 qed.
