proof/spec/Address.ec
@@ -119,7 +119,6 @@ op set_key_and_mask (address : adrs, key_and_mask : int) : adrs =
 
 op BytesToBits (bytes : W8.t list) : bool list = flatten (map W8.w2bits bytes).
 op BitsToBytes (bits : bool list) : W8.t list = map W8.bits2w (chunk W8.size bits).
-op W64ToBytes (w : W64.t, outlen : int) : W8.t list. (* = BitsToBytes (W64.w2bits w). *)
 
 op addr_to_bytes (a : W32.t Array8.t) : W8.t list = 
   let addr_bits : bool list = flatten (mkseq (fun (i : int) => W32.w2bits a.[i]) 8) in
