proof/spec/Hash.ec
@@ -18,10 +18,8 @@ op rand_hash_padding : W64.t = W64.one.
 op padding_len : int.
 axiom padding_len_ge0 : 0 <= padding_len.
 
-axiom size_hash (x : W8.t list) :  size (Hash x) = n. 
-
-op nbytexor(a b : nbytes) : nbytes = 
-    map (fun (ab : W8.t * W8.t) => ab.`1 `^` ab.`2) (zip a b).
+op bytexor(a b : W8.t list) : W8.t list = 
+   map (fun (ab : W8.t * W8.t) => ab.`1 `^` ab.`2) (zip a b).
 
 module Hash = {
   proc prf (in_0 : W8.t list, key : nbytes) : nbytes = {
@@ -30,7 +28,7 @@ module Hash = {
     var buf : W8.t list;
 
     padding <- take padding_len (W8u8.Pack.to_list (W8u8.unpack8 prf_padding_val));
-    buf <- padding ++ key ++ in_0;
+    buf <- padding ++ val key ++ in_0;
 
     r <- Hash buf;
 
@@ -44,7 +42,7 @@ module Hash = {
     var buf : W8.t list;
 
     padding <- take padding_len (W8u8.Pack.to_list (W8u8.unpack8 prf_padding_val));
-    buf <- padding ++ key ++ in_0;
+    buf <- padding ++ val key ++ in_0;
 
     r <- Hash buf;
     
@@ -59,7 +57,7 @@ module Hash = {
     var padding : W8.t list;
 
     padding <- take padding_len (W8u8.Pack.to_list (W8u8.unpack8 prf_padding_val));
-    buf <- padding ++ key ++ t;
+    buf <- padding ++ val key ++ val t;
 
     r <- Hash buf;
 
@@ -68,7 +66,7 @@ module Hash = {
 
   proc rand_hash (_left _right : nbytes, _seed : nbytes, address : adrs) : nbytes * adrs = {
       var padding : W8.t list;
-      var key : W8.t list;
+      var key : nbytes;
       var bitmask_0, bitmask_1 : nbytes;
       var buf, t : W8.t list; 
       var addr_bytes : W8.t list;
@@ -88,58 +86,10 @@ module Hash = {
       addr_bytes <- addr_to_bytes address;
       bitmask_1 <@ prf (addr_bytes,  _seed);
     
-      t <- nbytexor (_left ++ _right) (bitmask_0 ++ bitmask_1);
-      buf <- padding ++ key ++ t;
+      t <- bytexor (val _left ++ val _right) (val bitmask_0 ++ val bitmask_1);
+      buf <- padding ++ val key ++ t;
   
       return (Hash buf, address);
   }
 }.
 
-
-(*---------------------------------------------------------------------------------------------------------*)
-
-lemma prf_ll : islossless Hash.prf
-    by proc; wp; skip; smt(padding_len_ge0).
-
-lemma prf_kg_ll : islossless Hash.prf_keygen
-    by proc; wp; skip; smt(padding_len_ge0).
-
-lemma f_ll : islossless Hash._F 
-    by proc; wp; skip; smt(padding_len_ge0).
-
-lemma rand_hash_ll : islossless Hash.rand_hash
-    by proc; wp; do ! (call prf_ll; wp); skip; smt(padding_len_ge0).
-
-(*---------------------------------------------------------------------------------------------------------*)
-
-lemma _prf_size : hoare [Hash.prf : true ==> size res = n].
-proof.
-proc; seq 2 : (true); auto => />; smt(size_hash).
-qed.
-
-lemma prf_size : phoare [Hash.prf : true ==> size res = n] = 1%r 
-    by conseq prf_ll _prf_size => /#.
-
-lemma _prf_keygen_size : hoare [Hash.prf_keygen : true ==> size res = n].
-proof.
-proc; seq 2 : (true); auto => />; smt(size_hash).
-qed.
-
-lemma prf_keygen_size : phoare [Hash.prf_keygen : true ==> size res = n] = 1%r 
-    by conseq prf_kg_ll _prf_keygen_size => /#.
-
-lemma _f_size : hoare [Hash._F : true ==> size res = n].
-proof.
-proc; seq 2 : (true); auto => />; smt(size_hash).
-qed.
-
-lemma f_size : phoare [Hash._F : true ==> size res = n] = 1%r
-    by conseq f_ll _f_size => /#.
-
-lemma _randhash_size : hoare [Hash.rand_hash : true ==> size res.`1 = n]
-    by proc; seq 12 : (true); [ auto => /> | skip => />; by rewrite size_hash ].
-
-lemma randhash_size : phoare [Hash.rand_hash : true ==> size res.`1 = n] = 1%r
-    by conseq rand_hash_ll _randhash_size => /#.
-
-(*---------------------------------------------------------------------------------------------------------*)
