proof/spec/LTree.ec
@@ -15,7 +15,15 @@ op H_msg : threen_bytes -> W8.t list -> nbytes.
 clone export Subtype as WOTSKeys with 
    type T = wots_sk list,
    op P = fun l => size l = 2^h
-   rename "T" as "wots_keys".
+   rename "sT" as "wots_keys".
+
+clone export Subtype as AuthPath with
+  type T = nbytes list,
+  op P = fun l => size l = h
+  rename "sT" as "auth_path"
+  proof inhabited by (exists (nseq h witness);smt(size_nseq ge0_h))
+  proof *.
+
 
 (* 4.1.5 L-Trees *)
 (* takes as input a WOTS+ public key pk and compresses it to a single 
@@ -23,28 +31,31 @@ clone export Subtype as WOTSKeys with
 *)
 module LTree = {
   proc ltree (pk : wots_pk, address : adrs, _seed : seed) : nbytes * adrs = {
+    var pks : nbytes list;
     var pk_i : nbytes;
     var tmp : nbytes;
-    var i : int <- witness;
-    var _len : int <- len;
+    var i : int;
+    var _len : int;
     var tree_height : int;
 
     address <- set_tree_height address 0;
+    pks <- val pk;
 
+    _len <- len;
     while (1 < _len) { (* Same as _len > 1 *)
       i <- 0;
       while (i < _len %/ 2) {
         address <- set_tree_index address i;
-        pk_i <- nth witness pk (2*i);
-        tmp <- nth witness pk (2*i + 1);
+        pk_i <- nth witness pks (2*i);
+        tmp <- nth witness pks (2*i + 1);
         (pk_i, address) <@ Hash.rand_hash (pk_i, tmp, _seed, address);
-        pk <- put pk i pk_i;
+        pks <- put pks i pk_i;
         i <- i + 1;
       }
 
       if (_len %% 2 = 1) {
-        pk_i <- nth witness pk (_len - 1);
-        pk <- put pk (_len %/ 2) pk_i;
+        pk_i <- nth witness pks (_len - 1);
+        pks <- put pks (_len %/ 2) pk_i;
       }
 
       _len <- if _len %% 2 = 0 then _len %/ 2 else _len %/ 2 + 1;
@@ -53,15 +64,12 @@ module LTree = {
       address <- set_tree_height address (tree_height + 1);
     }
 
-    pk_i <- nth witness pk 0;
+    pk_i <- nth witness pks 0;
 
     return (pk_i, address);
   }
 }. 
 
-
-lemma ltree_ll : islossless LTree.ltree.
-admitted.
 
 (******************************************************************************)
 
