proof/spec/WOTS.ec
@@ -26,7 +26,9 @@ type wots_keypair = wots_pk * wots_sk.
 clone import Subtype as OTSKeys with 
    type T = wots_sk list,
    op P = fun l => size l = 2^h
-   rename "T" as "wots_ots_keys".
+   rename "sT" as "wots_ots_keys".
+
+op nbytexor(a b : nbytes) : nbytes =   NBytes.insubd (bytexor (val a) (val b)).
 
 module Chain = {
    proc chain(X : nbytes, i s : int, _seed : seed, address : adrs) : nbytes * adrs = {
@@ -70,9 +72,12 @@ pred chain_pre(X : nbytes, i s : int, _seed : seed, address : adrs) =
 module WOTS = {
   (* In practise, we generate the private key from a secret seed *)
   proc genSK() : wots_sk = {
-    var sk : wots_sk <- nseq len (nseq n W8.zero);
-    var sk_i : nbytes;
-    var i : int <- 0;
+    var sk : W8.t list list;
+    var sk_i : W8.t list;
+    var i : int;
+
+    sk <-(nseq len (nseq n W8.zero));
+    i <- 0;
 
     while (i < len) {
       sk_i <$ DList.dlist W8.dword n; (* Initialize sk[i] with a uniformly random n-byte string *)
@@ -80,7 +85,7 @@ module WOTS = {
       i <- i + 1;
     }
 
-    return sk;
+    return insubd (map NBytes.insubd sk);
   }
 
   (* 
@@ -98,11 +103,13 @@ module WOTS = {
 
   *)
   proc pseudorandom_genSK(sk_seed : nbytes, seed : nbytes, address : adrs) : wots_sk * adrs= {
-    var sk : wots_sk <- nseq len (nseq n witness);
+    var sk : nbytes list;
     var sk_i : nbytes;
     var addr_bytes : W8.t list;
     var buf : W8.t list;
     var i : int;
+
+    sk <-  nseq len witness;
     
     address <- set_hash_addr address 0;
     address <- set_key_and_mask address 0;
@@ -111,49 +118,56 @@ module WOTS = {
     while (i < len) {
       address <- set_chain_addr address i;
       addr_bytes <- addr_to_bytes address;
-      sk_i <@ Hash.prf_keygen (seed ++ addr_bytes, sk_seed);
+      sk_i <@ Hash.prf_keygen (val seed ++ addr_bytes, sk_seed);
       sk <- put sk i sk_i;
       i <- i + 1;
     }
 
-    return (sk, address);
+    return (insubd sk, address);
   }
 
   (* The len n-byte strings in the private key each define the start node for one hash chain. The public
   key consists of the end nodes of these hash chains *)
   proc genPK(sk : wots_sk, _seed : seed, address : adrs) : wots_pk * adrs = {
-    var pk : wots_pk <- nseq len (nseq n W8.zero);
-    var i : int <- 0;
-    var pk_i, sk_i : nbytes <- nseq n W8.zero;
+    var pk : nbytes list;
+    var i : int;
+    var pk_i, sk_i : nbytes;
+
+    pk <- nseq len witness;
+    i <- 0;
 
     while (i < len) {
       address <- set_chain_addr address i;
-      sk_i <- nth witness sk i;
+      sk_i <- nth witness (val sk) i;
       (pk_i, address) <@ Chain.chain (sk_i, 0, (w - 1), _seed, address);
       pk <- put pk i pk_i;
       i <- i + 1;
     }
 
-    return (pk, address);
+    return (insubd pk, address);
   }
 
   (* Generates the key from the seed *)
   proc pkGen(sk_seed : nbytes, _seed : seed, address : adrs) : wots_pk * adrs = {
-    var pk : wots_pk <- nseq len (nseq n W8.zero);
-    var wots_skey : wots_sk <- nseq len (nseq n W8.zero);
-    var i : int <- 0;
-    var pk_i, sk_i : nbytes <- nseq n W8.zero;
+    var pk : nbytes list;
+    var wots_skey : wots_sk;
+    var i : int;
+    var pk_i, sk_i : nbytes;
+
+    pk <- nseq len witness;
+    i <- 0;
+   
 
     (wots_skey, address) <@ pseudorandom_genSK(sk_seed, _seed, address); (* Generate sk from the secret key *)
     while (i < len) {
       address <- set_chain_addr address i;
-      sk_i <- nth witness wots_skey i;
+      sk_i <- nth witness (val wots_skey) i;
       (pk_i, address) <@ Chain.chain (sk_i, 0, (w - 1), _seed, address);
       pk <- put pk i pk_i;
       i <- i + 1;
     }
 
-    return (pk, address);
+    return (insubd pk, address);
   }
 
   proc kg(sk_seed : nbytes, _seed : seed, address : adrs) : wots_keypair = {
@@ -199,6 +213,7 @@ module WOTS = {
 
                                 WOTS+ Signature
   *)
+
   proc sign(M : wots_message, sk : wots_sk, _seed : seed, address : adrs) : wots_signature * adrs = {
     var csum_32 : W32.t;
     var csum : int;
@@ -208,14 +223,14 @@ module WOTS = {
     var len_2_bytes : int;
     var csum_bytes : W8.t list;
     var csum_base_w : int list;
-    var sig : wots_signature;
+    var sig : nbytes list;
     var sig_i : nbytes;
     var i : int;
 
-    sig <- nseq len (nseq n W8.zero);
+    sig <- nseq len witness;
 
     (* Convert message to base w *)
-    msg <@ BaseW.base_w(M, len1);
+    msg <@ BaseW.base_w(val M, len1);
 
     (* Compute checksum *)
     csum <@ checksum(msg);
@@ -234,13 +249,13 @@ module WOTS = {
     while (i < len) {
       address <- set_chain_addr address i;
       msg_i <- nth witness msg i;
-      sk_i <- nth witness sk i;
+      sk_i <- nth witness (val sk) i;
       (sig_i, address) <@ Chain.chain (sk_i, 0, msg_i, _seed, address);
       sig <- put sig i sig_i;
       i <- i + 1;
     }
 
-    return (sig, address);
+    return (insubd sig, address);
   }
 
   proc sign_seed (M : W8.t list, sk_seed : seed, pub_seed : seed, address : adrs) : wots_signature * adrs = {
@@ -253,11 +268,11 @@ module WOTS = {
     var len_2_bytes : int;
     var csum_bytes : W8.t list;
     var csum_base_w : int list;
-    var sig : wots_signature;
+    var sig : nbytes list;
     var sig_i : nbytes;
     var i : int;
 
-    sig <- nseq len (nseq n W8.zero);
+    sig <- nseq len witness;
 
     (* Generate sk from the secret seed *)
     (wots_skey, address) <@ pseudorandom_genSK(sk_seed, pub_seed, address); 
@@ -282,17 +297,17 @@ module WOTS = {
     while (i < len) {
       address <- set_chain_addr address i;
       msg_i <- nth witness msg i;
-      sk_i <- nth witness wots_skey i;
+      sk_i <- nth witness (val wots_skey) i;
       (sig_i, address) <@ Chain.chain (sk_i, 0, msg_i, pub_seed, address);
       sig <- put sig i sig_i;
       i <- i + 1;
     }
 
-    return (sig, address);
+    return (insubd sig, address);
   }
 
   proc pkFromSig(M : wots_message, sig : wots_signature, _seed : seed, address : adrs) : wots_pk * adrs = {
-    var tmp_pk : wots_pk <- nseq len (nseq n W8.zero);
+    var tmp_pk : nbytes list;
     var csum_32 : W32.t;
     var csum : int;
     var msg : int list;
@@ -304,8 +319,9 @@ module WOTS = {
     var msg_i : int;
     var pk_i : nbytes;
 
+    tmp_pk <-  nseq len witness;
     (* Convert message to base w *)
-    msg <@ BaseW.base_w(M, len1);
+    msg <@ BaseW.base_w(val M, len1);
 
     (* Compute checksum *)
     csum <@ checksum(msg);
@@ -324,13 +340,13 @@ module WOTS = {
     while (i < len) {
       address <- set_chain_addr address i;
       msg_i <- nth witness msg i;
-      sig_i <- nth witness sig i;
+      sig_i <- nth witness (val sig) i;
       (pk_i, address) <@ Chain.chain (sig_i, msg_i, (w - 1 - msg_i), _seed, address);
       tmp_pk <- put tmp_pk i pk_i; 
       i <- i + 1;
     }
 
-    return (tmp_pk, address);
+    return (insubd tmp_pk, address);
   }
 
   proc verify(pk : wots_pk, M : wots_message, sig : wots_signature, _seed : seed, address : adrs) : bool = {
@@ -340,99 +356,3 @@ module WOTS = {
   }
 }.
 
-(**********************************************************************************************************************)
-
-(* RFC - p 17
-Note that the checksum may reach a maximum integer value of len_1 * (w - 1) * 2^8.
-For the parameter sets specified in the RFC, a  32-bit unsigned integer is sufficient 
-to hold the checksum.
-*)
-
-axiom checksum_max : hoare[WOTS.checksum : true ==> res <= len1 * (w - 1) * 2^8].
-axiom checksum_W32 : hoare[WOTS.checksum : true ==> res <= W32.max_uint].
-
-(********************************************************************************************************************)
-
-lemma wots_genSK_ll : islossless WOTS.genSK
-    by proc; while (true) (len - i) ; auto => />; [ smt(@Distr @DList @W8) | smt() ].
-
-
-lemma wots_genSK_prf_ll : islossless WOTS.pseudorandom_genSK.
-proof.
-proc; wp; sp.
-while (true) (len - i) ; auto => />; [ sp; call prf_kg_ll; skip => /> /# | smt() ]. 
-qed.
-
-lemma chain_ll : islossless Chain.chain.
-proof.
-proc.
-while (true) (s - chain_count); last by auto => /> /#.
-auto => />.
-call f_ll; call prf_ll.
-wp.
-call prf_ll; auto => /#. 
-qed.
-
-lemma spec_base_w_ll : islossless BaseW.base_w.
-proof.
-proc.
-islossless.
-while (true) (outlen - consumed) ; by auto => /> /#.
-qed.
-
-lemma wots_genPK_ll : islossless WOTS.genPK.
-proof.
-proc ; islossless.
-while (true) (len - i) ; auto => />.
-  - call (chain_ll) ; auto => /> /#.
-  - smt().
-qed.
-
-lemma wots_pkGen_ll : islossless WOTS.pkGen.
-proof.
-proc.
-while (true) (len - i) ; auto => />.
-  - call (chain_ll) ; auto => /> /#.
-  - call (wots_genSK_prf_ll) ; auto => /#.
-qed.
-
-lemma wots_kg_ll : islossless WOTS.kg by proc ; call (wots_genPK_ll) ; call (wots_genSK_prf_ll).
-
-lemma wots_checksum_ll : islossless WOTS.checksum. 
-proof.
-proc.
-while (true) (len1 - i) ; by auto => /> /#.
-qed.
-
-lemma wots_sign_ll : islossless WOTS.sign.
-proof.
-proc.
-while (true) (len - i) ; auto => />.
-    - wp ; call (chain_ll) ; auto => /> /#.
-    - wp ; call (spec_base_w_ll). 
-      wp ; call (wots_checksum_ll). 
-      wp ; call (spec_base_w_ll). auto => /> /#.
-qed.
-
-lemma wots_sign_seed_ll : islossless WOTS.sign_seed.
-proof.
-proc.
-while (true) (len - i) ; auto => />.
-  - call chain_ll ; auto => /#.
-  - call (spec_base_w_ll) ; auto => />. 
-    call (wots_checksum_ll) ; auto => />.
-    call (spec_base_w_ll) ; auto => />.
-    call (wots_genSK_prf_ll) ; auto => /#.
-qed.
-
-lemma wots_pkFromSig_ll : islossless WOTS.pkFromSig.
-proof.
-proc.
-while (true) (len - i) ; auto => />.
-  - call (chain_ll) ; auto => /> /#.
-  - wp ; call (spec_base_w_ll).
-    wp ; call (wots_checksum_ll) ; call (spec_base_w_ll).
-    auto => /> /#.
-qed.
-
-lemma wots_verify_ll : islossless WOTS.verify by proc ; call (wots_pkFromSig_ll).
