proof/spec/xmss/XMSS_Types.ec
@@ -1,41 +1,15 @@
 require import AllCore List RealExp IntDiv.
 require (*  *) Subtype. 
 
-require export XMSS_Params WOTS.
+require export XMSS_Params WOTS Types.
 
 from Jasmin require import JModel.
 
 require import Array8.
 import Params.
 
-(* Same as single tree variant *)
-type xmss_sk = { idx : W32.t ;
-                 sk_seed : nbytes ; (* secret *)
-                 sk_prf : nbytes ;
-                 pub_seed_sk : nbytes ; (* public *)
-                 sk_root : nbytes }.
-
-(* Same as single tree variant *)
-type xmss_pk = { pk_oid : W32.t ;
-                 pk_root : nbytes ;
-                 pk_pub_seed : nbytes }.
-
-type msg_t = W8.t list.
-
-(* treeheight . n *)
-clone export Subtype as AuthPath with
-  type T = nbytes list,
-  op P = fun l => size l = 1
-  rename "T" as "auth_path"
-  proof inhabited by (exists [witness];auto)
-  proof *.
-
-type reduced_signature = wots_signature * auth_path.
-
 type sig_t = { sig_idx : W32.t;
                r : nbytes ;
-               r_sigs : reduced_signature list }.
-
-type xmss_keypair = xmss_sk * xmss_pk.
+               r_sig : reduced_signature }.
 
 (******************************************************************************)
