proof/spec/xmss_mt/XMSS_MT_TreeHash.ec
@@ -6,7 +6,7 @@ require (*--*) Subtype.
 
 from Jasmin require import JModel.
  
-require import XMSS_MT_Types Address Hash LTree WOTS.
+require import Types XMSS_MT_Types Address Hash LTree WOTS.
 import XMSS_MT_Params Params.
 
 (**********************************************************************************************)
@@ -27,7 +27,7 @@ pred treehash_p (s t : int) = s %% (1 `<<` t) <> 0.
 module TreeHash = {
   (* Computes the root *)
   proc treehash(pub_seed sk_seed : seed, s t : int, address : adrs) : nbytes * adrs = {
-  var node : nbytes <- nseq n W8.zero;
+  var node : nbytes <- witness;
   var stack : nbytes list <- [];
   var top_node : nbytes;
   var pk : wots_pk;
@@ -88,26 +88,18 @@ module TreeHash = {
   }
 }.
 
-lemma treehash_ll : islossless TreeHash.treehash.
-proof.
-proc.
-sp ; wp.
-while (true) (2^t - i); last by skip => /> /#.
-auto => />. sp.
-while (true) (offset - 1).
-  + auto => />; call rand_hash_ll; wp; skip => /> /#.
-  + wp; call ltree_ll; wp; call wots_pkGen_ll; wp. skip => /> *.
-    split; [ move => *; rewrite negb_and; left |]; smt().
-qed.
 
 module TreeSig = {
   (* Compute the authentication path for the i-th WOTS+ key pair *)
   proc buildAuthPath(pub_seed sk_seed : seed, idx : W32.t, address : adrs) : auth_path * adrs = {
-    var authentication_path : auth_path <- nseq len (nseq n W8.zero);
-    var j : int <- 0;
+    var authentication_path : nbytes list;
+    var j : int ;
     var k : int;
     var t : nbytes <- witness;
 
+    authentication_path <- nseq len witness;
+
+    j <- 0;
     while (j < h) {
       k <- floor((W32.to_uint idx)%r / (2^j)%r);
       (t, address) <@ TreeHash.treehash(pub_seed, sk_seed , k * (2^j), j, address);
@@ -115,12 +107,12 @@ module TreeSig = {
       j <- j + 1;
     }
 
-    return (authentication_path, address);
+    return (AuthPath.insubd authentication_path, address);
   }
 
   (* Generate a WOTS+ signature on a message with corresponding authentication path *)
   proc treesig(M : nbytes, pub_seed sk_seed : seed, idx : W32.t, address : adrs) : wots_signature * auth_path * adrs  = {
-    var auth : auth_path <- nseq len (nseq n W8.zero);
+    var auth : auth_path;
     var sig_ots : wots_signature;
     var ots_sk : wots_sk;
     var seed : nbytes;
@@ -129,20 +121,11 @@ module TreeSig = {
     address <- set_type address 0;
     address <- set_ots_addr address (W32.to_uint idx);
 
-    (sig_ots, address) <@ WOTS.sign_seed(M, sk_seed, pub_seed, address);
+    (sig_ots, address) <@ WOTS.sign_seed(val M, sk_seed, pub_seed, address);
     
     return (sig_ots, auth, address);
   }
 }.
-
-lemma buildAuthPath_ll : islossless TreeSig.buildAuthPath.
-proof.
-proc.
-while (0 <= j <= h) (h - j) ; auto => />; [call treehash_ll ; auto => /> /# | smt(h_g0) ]. 
-qed.
-
-lemma treesig_ll : islossless TreeSig.treesig
-    by proc; call wots_sign_seed_ll; auto => /> ; call buildAuthPath_ll; auto.
 
 (**********************************************************************************************)
 
@@ -182,13 +165,13 @@ module RootFromSig = {
         index <- get_tree_index address;
         address <- set_tree_index address (index %/ 2);
 
-        auth_k <- nth witness auth k;
+        auth_k <- nth witness (val auth) k;
         (nodes1, address) <@ Hash.rand_hash (nodes0, auth_k, _seed, address);
       } else {
         index <- get_tree_index address;
         address <- set_tree_index address ((index - 1) %/ 2);
 
-        auth_k <- nth witness auth k;
+        auth_k <- nth witness (val auth) k;
         (nodes1, address) <@ Hash.rand_hash (auth_k, nodes0, _seed, address);
       }
 
@@ -199,16 +182,3 @@ module RootFromSig = {
     return nodes0;
   }
 }.
-
-lemma root_from_sig_ll : islossless RootFromSig.rootFromSig.
-proof.
-proc.
-while (0 <= k <= h) (h - k) ; auto => />.
-  + wp; sp. if. 
-      * call rand_hash_ll. islossless. auto => /> &hr *; do split; admit. 
-      * call rand_hash_ll. islossless. auto => /> &hr *; do split; admit.
-  + auto => />; do split => /#.
-  + call ltree_ll ; auto => />. 
-    call wots_pkFromSig_ll ; auto => />.
-    smt(h_g0).
-qed.
