proof/spec/xmss_mt/XMSS_MT_Types.ec
@@ -1,43 +1,16 @@
 require import AllCore List RealExp IntDiv.
 require (*  *) Subtype. 
 
-require import XMSS_MT_Params WOTS.
+require import XMSS_MT_Params Types WOTS.
 
 from Jasmin require import JModel.
 
 require import Array8.
 
-
-(* treeheight . n *)
-clone export Subtype as AuthPath with
-  type T = nbytes list,
-  op P = fun l => size l = d
-  rename "T" as "auth_path"
-  proof inhabited by (exists (mkseq (fun i => witness) d);rewrite /P size_mkseq;smt(ge0_d))
-  proof *.
-
 (******************************************************************************)
-
-(* Same as single tree variant *)
-type xmss_mt_sk = { idx : W32.t ;
-                    sk_seed : nbytes ; (* secret *)
-                    sk_prf : nbytes ;
-                    pub_seed_sk : nbytes ; (* public *)
-                    sk_root : nbytes }.
-
-(* Same as single tree variant *)
-type xmss_mt_pk = { pk_oid : W32.t ;
-                    pk_root : nbytes ;
-                    pk_pub_seed : nbytes }.
-
-type msg_t = W8.t list.
-
-type reduced_signature = wots_signature * auth_path.
 
 type sig_t = { sig_idx : W32.t;
                r : nbytes ;
                r_sigs : reduced_signature list }.
-
-type xmss_mt_keypair = xmss_mt_sk * xmss_mt_pk.
 
 (******************************************************************************)
